celliocb/MaincbHeader.v
@@ -3,4 +3,5 @@ Require Import CRIS.
 Module MaincbHdr.
   Definition input_stdin : string := "Input_stdin".
   Definition input_db : string := "Input_db".
+  Definition input_cb : string := "Input_cb".
 End MaincbHdr.
